LeanHoG/Invariant/ConnectedComponents/Certificate.lean
@@ -6,7 +6,6 @@ import LeanHoG.Invariant.ConnectedComponents.Basic
 import LeanHoG.Util.Quote
 import LeanHoG.Util.RB
 import LeanHoG.Certificate
-import Std
 
 open Qq
 
@@ -18,23 +17,23 @@ def connectedComponentsCertificateOfData (G : Q(Graph)) (C : ConnectedComponents
   have zeroVal : Q(Fin $val) := finOfData val 0
   have zeroVert : Q(Graph.vertex $G) := finOfData n 0
   have convertToPairFinVal : Nat × Nat → Q(Fin $n × Fin $val) := fun (i,j) => q(($(finOfData n i), $(finOfData val j)))
-  have componentMap : Q(Std.RBMap (Graph.vertex $G) (Fin $val) Fin.instLinearOrderFin.compare) :=
-    build_RBMap (C.component.map convertToPairFinVal) q(Fin.instLinearOrderFin)
-  have component : Q(Graph.vertex $G → Fin $val) := q(fun v => Std.RBMap.findD $componentMap v $zeroVal)
-  have componentEdge : Q(Std.RBSet.all (Graph.edgeSet $G) (fun x => $component (Graph.fst x) = $component (Graph.snd x)) = true) := (q(Eq.refl true) : Lean.Expr)
+  have componentMap : Q(Batteries.RBMap (Graph.vertex $G) (Fin $val) Fin.instLinearOrder.compare) :=
+    build_RBMap (C.component.map convertToPairFinVal) q(Fin.instLinearOrder)
+  have component : Q(Graph.vertex $G → Fin $val) := q(fun v => Batteries.RBMap.findD $componentMap v $zeroVal)
+  have componentEdge : Q(Batteries.RBSet.all (Graph.edgeSet $G) (fun x => $component (Graph.fst x) = $component (Graph.snd x)) = true) := (q(Eq.refl true) : Lean.Expr)
   have convertToPairValFin : Nat × Nat → Q(Fin $val × Fin $n) := fun (i,j) => q(($(finOfData val i), $(finOfData n j)))
-  have rootMap : Q(Std.RBMap (Fin $val) (Graph.vertex $G) Fin.instLinearOrderFin.compare) :=
-    build_RBMap (C.root.map convertToPairValFin) q(Fin.instLinearOrderFin)
-  have root : Q(Fin $val → Graph.vertex $G) := q(fun v => Std.RBMap.findD $rootMap v $zeroVert)
+  have rootMap : Q(Batteries.RBMap (Fin $val) (Graph.vertex $G) Fin.instLinearOrder.compare) :=
+    build_RBMap (C.root.map convertToPairValFin) q(Fin.instLinearOrder)
+  have root : Q(Fin $val → Graph.vertex $G) := q(fun v => Batteries.RBMap.findD $rootMap v $zeroVert)
   have rootCorrect : Q(forallFin (fun i => $component ($root i) = i) = true) := (q(Eq.refl true) : Lean.Expr)
   have convertToPairOfFins : Nat × Nat → Q(Fin $n × Fin $n) := fun (i,j) => q(($(finOfData n i), $(finOfData n j)))
-  have nextMap : Q(Std.RBMap (Graph.vertex $G) (Graph.vertex $G) Fin.instLinearOrderFin.compare) :=
-    build_RBMap (C.next.map convertToPairOfFins) q(Fin.instLinearOrderFin)
-  have next : Q(Graph.vertex $G → Graph.vertex $G) := q(fun v => Std.RBMap.findD $nextMap v v)
+  have nextMap : Q(Batteries.RBMap (Graph.vertex $G) (Graph.vertex $G) Fin.instLinearOrder.compare) :=
+    build_RBMap (C.next.map convertToPairOfFins) q(Fin.instLinearOrder)
+  have next : Q(Graph.vertex $G → Graph.vertex $G) := q(fun v => Batteries.RBMap.findD $nextMap v v)
   have convertToFinNat : Nat × Nat → Q(Fin $n × Nat) := fun (i,j) => q(($(finOfData n i), $j))
-  have distToRootMap : Q(Std.RBMap (Graph.vertex $G) Nat Fin.instLinearOrderFin.compare) :=
-    build_RBMap (C.distToRoot.map convertToFinNat) q(Fin.instLinearOrderFin)
-  have distToRoot : Q(Graph.vertex $G → Nat) := q(fun v => Std.RBMap.findD $distToRootMap v 0)
+  have distToRootMap : Q(Batteries.RBMap (Graph.vertex $G) Nat Fin.instLinearOrder.compare) :=
+    build_RBMap (C.distToRoot.map convertToFinNat) q(Fin.instLinearOrder)
+  have distToRoot : Q(Graph.vertex $G → Nat) := q(fun v => Batteries.RBMap.findD $distToRootMap v 0)
   have distRootZero : Q(forallFin (fun i => $distToRoot ($root i) = 0) = true) := (q(Eq.refl true) : Lean.Expr)
   have distZeroRoot : Q(forallVertex (fun (v : Graph.vertex $G) => $distToRoot v = 0 → v = $root ($component v)) = true) := (q(Eq.refl true) : Lean.Expr)
   have nextRoot : Q(forallFin (fun i => $next ($root i) = $root i) = true) := (q(Eq.refl true) : Lean.Expr)
