LeanHoG/Invariant/G6.lean
@@ -3,7 +3,7 @@ import LeanHoG.Graph
 
 namespace LeanHoG
 
-class G6 (G : Graph) : Type :=
+class G6 (G : Graph) : Type where
   val : String
 
 def Graph.g6 {G : Graph} [g6 : G6 G] : String := g6.val
