LeanHoG/Invariant/HamiltonianPath/SatHelpers.lean
@@ -1,9 +1,9 @@
-import LeanSAT
+import Trestle.Model.PropFun
 
 namespace LeanHoG
 namespace PropFun
 
-open LeanSAT Model PropFun
+open Trestle Model PropFun
 
 @[simp]
 def disj_list {ν : Type} : List (PropFun ν) → PropFun ν
@@ -17,7 +17,7 @@ def satisfies_disj_list_to_witness {ν : Type} {τ : PropAssignment ν} (ps : Li
   | p :: ps => by
     simp at h
     if τ_sat_p : τ ⊨ p then
-      exact ⟨p, ⟨List.mem_cons_self _ _, τ_sat_p⟩⟩
+      exact ⟨p, ⟨List.mem_cons_self, τ_sat_p⟩⟩
     else
       simp [τ_sat_p] at h
       let ⟨p', ⟨p'_mem, τ_sat_p'⟩⟩ := satisfies_disj_list_to_witness ps h
@@ -27,30 +27,37 @@ lemma satisfies_disj_list {ν : Type} {τ : PropAssignment ν} {ps : List (PropF
   τ ⊨ (disj_list ps) ↔ ∃ p ∈ ps, τ ⊨ p := by
   apply Iff.intro
   · intro h
-    induction' ps with p ps ih
-    · contradiction
-    · simp at h
-      cases' h with h h
-      · apply Exists.intro p
+    induction ps with --p ps ih
+    | nil => contradiction
+    | cons p ps ih =>
+      simp at h
+      cases h with
+      | inl h =>
+        apply Exists.intro p
         simp
         assumption
-      · have := ih h
+      | inr h =>
+        have := ih h
         let ⟨p, p_in_ps, sat⟩ := this
         apply Exists.intro p
         simp [p_in_ps]
         assumption
   · intro h
-    induction' ps with q qs ih
-    · let ⟨p, _, _⟩ := h
+    induction ps with
+    | nil =>
+      let ⟨p, _, _⟩ := h
       contradiction
-    · let ⟨p, p_in_ps, sat⟩ := h
+    | cons q qs ih =>
+      let ⟨p, p_in_ps, sat⟩ := h
       simp
       simp at p_in_ps
-      cases' p_in_ps with p_eq_q
-      · apply Or.intro_left
+      cases p_in_ps with
+      | inl p_eq_q =>
+        apply Or.intro_left
         rw [← p_eq_q]
         assumption
-      · apply Or.intro_right
+      | inr _ =>
+        apply Or.intro_right
         apply ih
         apply Exists.intro p
         apply And.intro
@@ -64,8 +71,8 @@ def conj_list {ν : Type} : List (PropFun ν) → PropFun ν
 
 lemma satisfies_conj_list {ν : Type} {τ : PropAssignment ν} {ps : List (PropFun ν)} :
   τ ⊨ (conj_list ps) ↔ ∀ p ∈ ps, τ ⊨ p := by
-  induction' ps with q qs ih
-  simp_all only [conj_list, satisfies_tr, List.find?_nil, List.not_mem_nil, IsEmpty.forall_iff, forall_const]
+  induction ps
+  simp_all only [conj_list, List.not_mem_nil, IsEmpty.forall_iff, forall_const]
   · simp
     rfl
   · simp_all [conj_list, satisfies_conj, List.mem_cons, forall_eq_or_imp]
@@ -75,9 +82,9 @@ lemma satisfies_disj_fls {ν : Type} {τ : PropAssignment ν} {p : PropFun ν} :
   apply Iff.intro
   · intro h
     simp at h
-    cases' h with h h'
-    exact h
-    contradiction
+    cases h with
+    | inl h => exact h
+    | inr _ => contradiction
   · intro h
     simp
     apply Or.intro_left
