LeanHoG/Invariant/NeighborhoodMap/Basic.lean
@@ -1,4 +1,4 @@
-import Std.Data.RBMap
+import Batteries.Data.RBMap
 import LeanHoG.Graph
 import LeanHoG.Edge
 import LeanHoG.Util.RB
@@ -8,11 +8,11 @@ namespace LeanHoG
 @[reducible]
 def edgeCorrect (G : Graph) (M : G.vertexMap G.vertexSubset) :
   G.edgeType → Prop :=
-  fun e => (G.fst e) ∈ (M.findD (G.snd e) Std.RBSet.empty) ∧ (G.snd e) ∈ (M.findD (G.fst e) Std.RBSet.empty)
+  fun e => (G.fst e) ∈ (M.findD (G.snd e) Batteries.RBSet.empty) ∧ (G.snd e) ∈ (M.findD (G.fst e) Batteries.RBSet.empty)
 
 class NeighborhoodMap (G : Graph) where
   neighbors : G.vertexMap G.vertexSubset
-  neighbor_is_adjacent : ∀ (u : G.vertex), (neighbors.findD u Std.RBSet.empty).all (G.adjacent u)
+  neighbor_is_adjacent : ∀ (u : G.vertex), (neighbors.findD u Batteries.RBSet.empty).all (G.adjacent u)
   adjacent_is_neighbor : ∀ e : G.edge, edgeCorrect G neighbors e
 
 end LeanHoG
